books/centaur/misc/iffstar.lisp
@@ -33,26 +33,6 @@
 
 (in-package "ACL2")
 
+(include-book "starlogic")
 
-(include-book "std/util/define" :dir :system)
-
-
-;; IFF* is just like IFF, but doesn't automatically cause case splits.
-(define iff* (x y)
-  (iff x y)
-  ///
-  (defequiv iff*)
-  (defrefinement iff iff*)
-  (defrefinement iff* iff)
-  (defthm iff*-of-nonnils
-    (implies (and x y)
-             (equal (iff* x y) t))
-    :rule-classes ((:rewrite :backchain-limit-lst 0)))
-  (defthm iff*-with-nil
-    (and (equal (iff* x nil)
-                (not x))
-         (equal (iff* nil x)
-                (not x))))
-  (defthm iff*-with-t
-    (and (iff (iff* x t) x)
-         (iff (iff* t x) x))))
+; cert_param (reloc_stub)
